theories/TRAKHTENBROT/Sign_Sig2.v
@@ -1,0 +1,318 @@
+(**************************************************************)
+(*   Copyright Dominique Larchey-Wendling [*]                 *)
+(*                                                            *)
+(*                             [*] Affiliation LORIA -- CNRS  *)
+(**************************************************************)
+(*      This file is distributed under the terms of the       *)
+(*         CeCILL v2 FREE SOFTWARE LICENSE AGREEMENT          *)
+(**************************************************************)
+
+Require Import List Arith Bool Lia Eqdep_dec.
+
+From Undecidability.Shared.Libs.DLW.Utils
+  Require Import utils_tac utils_list utils_nat finite.
+
+From Undecidability.Shared.Libs.DLW.Vec 
+  Require Import pos vec.
+
+From Undecidability.Shared.Libs.DLW.Wf 
+  Require Import wf_finite.
+
+From Undecidability.TRAKHTENBROT
+  Require Import notations fol_ops fo_sig fo_terms fo_logic fo_sat
+                 membership hfs reln_hfs.
+
+Set Implicit Arguments.
+
+Local Notation ø := vec_nil.
+
+Section Sign_Sig2_encoding.
+
+  Variable (n : nat).
+
+  Notation Σ2 := (Σrel 2).
+  Notation Σn := (Σrel n).
+
+  Infix "∈" := Σ2_mem.
+  Infix "≈" := Σ2_equiv.
+  Infix "⊆" := Σ2_incl.
+
+  (* We bound quantification inside hf-set l ∈ p and r ∈ p represent a set 
+     of ordered triples corresponding to M3 *)
+
+  Fixpoint Σn_Σ2 (l r : nat) (A : fol_form Σn) : fol_form Σ2 :=
+    match A with
+      | ⊥             => ⊥
+      | fol_atom _  v => Σ2_is_tuple_in r (vec_map (@Σrel_var _) v)
+      | fol_bin b A B => fol_bin b (Σn_Σ2 l r A) (Σn_Σ2 l r B)
+      | fol_quant fol_fa A  => ∀ 0 ∈ (S l) ⤑ Σn_Σ2 (S l) (S r) A
+      | fol_quant fol_ex A  => ∃ 0 ∈ (S l) ⟑ Σn_Σ2 (S l) (S r) A
+     end.
+
+  Variable (X : Type) (M2 : fo_model Σ2 X).
+  Variable (Y : Type) (Mn : fo_model Σn Y).
+
+  Let mem a b := fom_rels M2 tt (a##b##ø).
+
+  Infix "∈m" := mem (at level 59, no associativity).
+  Notation P := (fun v => fom_rels Mn tt v).
+
+  Variable R : Y -> X -> Prop.
+
+  (** R represent a relation  Mn <~> M2 = { x | x ∈ p } which
+      ensures the soundness & completeness of the encoding
+      These are the conditions for correctness 
+
+      HR1 : R is onto from Mn to { x | x ∈ l }
+      HR2 : R is onto from { x | x ∈ l } to Mn
+      HR3 : R relates the n-ary relation in Mn 
+            and the n-ary relation <_,...,_> ∈ r in M2
+
+    *)
+
+  Let HR1 (l r : X) := forall y, exists x, x ∈m l /\ R y x.
+  Let HR2 (l r : X) := forall x, x ∈m l -> exists y, R y x.
+  Let HR3 (l r : X) := forall v w, (forall p, R (vec_pos v p) (vec_pos w p))
+         -> P v <-> mb_is_tuple_in mem r w.
+
+  Notation "⟪ A ⟫" := (fun ψ => fol_sem M2 ψ A).
+  Notation "⟪ A ⟫'" := (fun φ => fol_sem Mn φ A) (at level 1, format "⟪ A ⟫'").
+
+  (* The correctness lemma *)
+ 
+  Lemma Σn_Σ2_correct (A : fol_form Σn) l r φ ψ :
+            HR1 (ψ l) (ψ r) 
+         -> HR2 (ψ l) (ψ r) 
+         -> HR3 (ψ l) (ψ r)
+        -> (forall x, In x (fol_vars A) -> R (φ x) (ψ x))
+        -> ⟪ A ⟫' φ <-> ⟪Σn_Σ2 l r A⟫ ψ.
+  Proof.
+    revert l r φ ψ.
+    induction A as [ | [] | b A HA B HB | [] A HA ]; intros l r phi psy H1 H2 H3 H.
+    + simpl; tauto.
+    + simpl; red in H3.
+      rewrite H3 with (w := vec_map (fun x => psy (Σrel_var x)) v).
+      * apply (fol_quant_sem_ext fol_ex); intros x.
+        apply (fol_bin_sem_ext fol_conj); try tauto.
+        rewrite Σ2_is_tuple_spec; simpl.
+        rewrite !vec_map_map; simpl; tauto.
+      * intros p; rewrite !vec_pos_map.
+        case_eq (vec_pos v p).
+        2: intros [].
+        simpl; intros x Hx; rewrite Hx; simpl.
+        apply H; simpl; apply in_flat_map.
+        exists (vec_pos v p); split.
+        - apply in_vec_list, in_vec_pos.
+        - simpl; rewrite Hx; simpl; auto.
+    + simpl; apply fol_bin_sem_ext; [ apply HA | apply HB ];
+        intros; auto; apply H, in_or_app; simpl; auto.
+    + simpl; split.
+      * intros (x & Hx).
+        destruct (H1 x) as (y & G1 & G2).
+        exists y; split.
+        - rew fot; simpl; auto.
+        - revert Hx; apply HA; auto.
+          intros [ | n' ]; simpl; auto.
+          intros; apply H; simpl; apply in_flat_map; exists (S n'); simpl; auto.
+      * intros (y & G1 & G2); revert G1 G2; rew fot; simpl; intros G1 G2.
+        destruct (H2 _ G1) as (x & G3).
+        exists x; revert G2; apply HA; auto.
+        intros [ | n' ]; simpl; auto.
+        intros; apply H; simpl; apply in_flat_map; exists (S n'); simpl; auto.
+    + simpl; split.
+      * intros G1 y; rew fot; simpl; intros G2.
+        destruct (H2 _ G2) as (x & G3).
+        generalize (G1 x); apply HA; auto.
+        intros [ | n' ]; simpl; auto.
+        intros; apply H; simpl; apply in_flat_map; exists (S n'); simpl; auto.
+      * intros G1 x.
+        destruct (H1 x) as (y & G2 & G3).
+        generalize (G1 _ G2); apply HA; auto.
+        intros [ | n' ]; simpl; auto.
+        intros; apply H; simpl; apply in_flat_map; exists (S n'); simpl; auto.
+  Qed.
+
+  Variable A : fol_form Σn.
+
+  (** We make some space for l and r *)
+
+  Let B := fol_subst (fun v => £ (2+v)) A.
+  Let l := 0.
+  Let r := 1.
+
+  (* Notice that Σn_Σ2 A has two more free variables than A,
+     that could be quantified existentially over if needed *)
+
+  (** The FO set-theoretic axioms we need to add are somewhat minimal:
+         - ∈ must be extensional (of course, this is a set-theoretic model)
+         - ordered n-tuples encoded in the usual way should exists for elements ∈ l 
+         - l should not be the empty set 
+         - and free variables of A (lifted twice) should be interpreted in l
+   *)
+
+  Definition Σn_Σ2_enc := 
+                Σ2_extensional 
+              ⟑ Σ2_non_empty l
+              ⟑ Σ2_list_in l (fol_vars B) 
+              ⟑ Σn_Σ2 l r B.
+
+End Sign_Sig2_encoding.
+
+Section SAT2_SATn.
+
+  Variable n : nat.
+
+  (** We show the easy implication, any model of Σn_Σ2_enc A
+     gives rise to a model of A *)
+
+  Section nested.
+
+    Variables (A : fol_form (Σrel n))
+              (X : Type) 
+              (M2 : fo_model (Σrel 2) X)
+              (M2fin : finite_t X)
+              (M2dec : fo_model_dec M2)
+              (ψ : nat -> X)
+              (HA : fol_sem M2 ψ (Σn_Σ2_enc A)).
+
+    Let mem a b := fom_rels M2 tt (a##b##ø).
+
+    Let mem_dec : forall x y, { mem x y } + { ~ mem x y }.
+    Proof. intros x y; apply (@M2dec tt). Qed.
+
+    Let P x := (if mem_dec x (ψ 0) then true else false) = true.
+
+    Let HP0 x : P x <-> mem x (ψ 0).
+    Proof.
+      unfold P.
+      destruct (mem_dec x (ψ 0)); split; try tauto; discriminate.
+    Qed.
+
+    Let HP1 : finite_t (sig P).
+    Proof.
+      apply fin_t_finite_t.
+      + intros; apply UIP_dec, bool_dec.
+      + apply finite_t_fin_t_dec; auto.
+        intro; apply bool_dec.
+    Qed.
+
+    Let Mn : fo_model (Σrel n) (sig P).
+    Proof.
+      exists.
+      + intros [].
+      + intros [] v.
+        simpl in v.
+        apply (@mb_is_tuple_in _ mem (ψ 1) n).
+        apply (vec_map (@proj1_sig _ _) v).
+    Defined.
+
+    Let Mn_dec : fo_model_dec Mn.
+    Proof. intros [] v; apply mb_is_tuple_in_dec; auto. Qed.
+
+    Let R (x : sig P) (y : X) := proj1_sig x = y.
+
+    Local Lemma SAT2_to_SATn : exists Y, fo_form_fin_dec_SAT_in A Y.
+    Proof.
+      exists (sig P).
+      destruct HA as (H1 & H2 & H3 & H4).
+      rewrite Σ2_non_empty_spec in H2.
+      rewrite Σ2_list_in_spec in H3.
+      revert H3 H4; set (B := A⦃fun v : nat => in_var (2 + v)⦄); intros H3 H4.
+      assert (H5 : forall n, In n (fol_vars B) -> P (ψ n)).
+      { intros; apply HP0, H3; auto. }
+      destruct H2 as (x0 & H0).
+      generalize H0; intros H2.
+      apply HP0 in H0.
+      set (phi := fun n : nat => 
+        match in_dec eq_nat_dec n (fol_vars B) with 
+          | left H  => (exist _ (ψ n) (H5 _ H) : sig P)
+          | right _ => (exist _ x0 H0 : sig P)
+        end).
+      exists Mn, HP1, Mn_dec, (fun n => phi (2+n)).
+      unfold B in *; clear B.
+      rewrite <- Σn_Σ2_correct with (Mn := Mn) (φ := phi) (R := R) in H4.
+      + rewrite fol_sem_subst in H4.
+        revert H4; apply fol_sem_ext; intro; rew fot; auto.
+      + intros (x & Hx); exists x; unfold R; simpl; split; auto.
+        apply HP0 in Hx; auto.
+      + intros x Hx; apply HP0 in Hx.
+        exists (exist _ x Hx); red; simpl; auto.
+      + intros v w Hvw. simpl.
+        apply fol_equiv_ext; f_equal.
+        apply vec_pos_ext; intros p.
+        rewrite vec_pos_map; apply Hvw.
+      + intros j Hj; red.
+        unfold phi.
+        destruct (in_dec eq_nat_dec j (fol_vars A⦃fun v : nat => in_var (2 + v)⦄))
+          as [ H | [] ]; auto; simpl.
+    Qed.
+
+  End nested.
+
+  Theorem SAT2_SATn A : fo_form_fin_dec_SAT (@Σn_Σ2_enc n A)
+                     -> fo_form_fin_dec_SAT A.
+  Proof.
+    intros (X & M2 & H1 & H2 & psy & H3).
+    apply SAT2_to_SATn with X M2 psy; auto.
+  Qed.
+
+End SAT2_SATn.
+
+Section SATn_SAT2.
+
+  Variable n : nat.
+
+  (** This is the hard implication. From a model of A, 
+      build a model of Σn_Σ2_enc A in hereditary finite sets *)
+
+  Section nested.
+
+    Variables (A : fol_form (Σrel n))
+              (X : Type) (Mn : fo_model (Σrel n) X)
+              (X_fin : finite_t X)
+              (X_discr : discrete X)
+              (Mn_dec : fo_model_dec Mn)
+              (φ : nat -> X)
+              (HA : fol_sem Mn φ A).
+
+    Let R := fom_rels Mn tt.
+
+    Local Lemma SATn_to_SAT2 : exists Y, fo_form_fin_dec_SAT_in (@Σn_Σ2_enc n A) Y.
+    Proof.
+      destruct reln_hfs with (R := fom_rels Mn tt)
+        as (Y & H1 & H2 & mem & H3 & l & r & i & s & H4 & H5 & H6 & H7 & H8 & H9 & H10); auto.
+      exists Y, (bin_rel_Σ2 mem), H1, (bin_rel_Σ2_dec _ H3), 
+        (fun n => match n with 
+           | 0 => l
+           | 1 => r
+           | S (S n) => i (φ n)
+         end).
+      unfold Σn_Σ2_enc; msplit 3; auto.
+      + exists (i (φ 0)); simpl; rew fot; simpl; auto.
+      + apply Σ2_list_in_spec.
+        intros n'; simpl.
+        rewrite fol_vars_map, in_map_iff.
+        intros (m & <- & ?); auto.
+      + rewrite <- Σn_Σ2_correct with (Mn := Mn) (R := fun x y => y = i x) 
+            (φ := fun n => match n with 0 => φ 0 | 1 => φ 1 | S (S n) => φ n end); auto.
+        * rewrite fol_sem_subst.
+          revert HA; apply fol_sem_ext.
+          intros; simpl; rew fot; auto.
+        * intros x; exists (i x); split; auto; apply H6.
+        * intros v w E; rewrite H9.
+          apply fol_equiv_ext; f_equal.
+          apply vec_pos_ext; intro; rew vec.
+        * intros n'; rewrite fol_vars_map, in_map_iff.
+          intros (m & <- & Hm); simpl; auto.
+    Qed.
+
+  End nested.
+
+  Theorem SATn_SAT2 A : fo_form_fin_discr_dec_SAT A
+                     -> fo_form_fin_dec_SAT (@Σn_Σ2_enc n A).
+  Proof.
+    intros (X & H1 & Mn & H2 & H4 & psy & H5).
+    apply SATn_to_SAT2 with X Mn psy; auto.
+  Qed.
+
+End SATn_SAT2.
