theories/TRAKHTENBROT/reln_hfs.v
@@ -1,0 +1,450 @@
+(**************************************************************)
+(*   Copyright Dominique Larchey-Wendling [*]                 *)
+(*                                                            *)
+(*                             [*] Affiliation LORIA -- CNRS  *)
+(**************************************************************)
+(*      This file is distributed under the terms of the       *)
+(*         CeCILL v2 FREE SOFTWARE LICENSE AGREEMENT          *)
+(**************************************************************)
+
+Require Import List Arith Lia Eqdep_dec Bool.
+
+From Undecidability.Shared.Libs.DLW.Utils 
+  Require Import utils_tac utils_list finite.
+
+From Undecidability.Shared.Libs.DLW.Vec 
+  Require Import pos vec.
+
+From Undecidability.TRAKHTENBROT
+  Require Import notations fol_ops membership hfs.
+
+Set Implicit Arguments.
+
+Section bt_model_n.
+
+  (** This discussion briefly describes how we encode finite and discrete 
+      model X with a computable n-ary relation R into an hereditary finite 
+      set (hfs) with to elements l and r, l representing the points in X
+      and r representing the n-tuples in R.
+
+      Because X is finite and discrete, one can compute a bijection X <~> pos n
+      where n is the cardinal of X. Hence we assume that X = pos n and the
+      ternary relation is R : pos n -> pos n -> pos n -> Prop
+      
+      1) We find a transitive hfs l such that pos n bijects with the elements
+         of l (transitive means ∀x, x∈l -> x⊆l). Hence
+
+                            pos n <-> { x | x ∈ l } 
+
+         For this, we use the encoding of natural numbers into sets, 
+         ie 0 := ø and 1+i := {i} U i and choose l to be the encoding 
+         of n (the cardinal of X=pos n above).
+
+         Notice that since l is transitive then so is P(l) (powerset)
+         and hence P^i(l) for any i.
+    
+      2) forall x,y ∈ l, both {x} and {x,y} belong to P(l) 
+         hence (x,y) = {{x},{x,y}} ∈ P(P(l))=P^2(l)
+        
+      3) P^1(l) = P(l) contains the empty set
+  
+      4) Hence P^(2n+1)(l) contains all n-tuples build from the elements of l
+         by induction on n
+
+      5) So we can encode R as hfs r ∈ p := P^(2n+2)(l) = P(P^(2n+1)(l)) and
+         p serves as our model, ie 
+
+                      Y := { x : hfs | x ∈b p } 
+
+         where x ∈b p is the Boolean encoding of x ∈ p to ensure 
+         uniqueness of witnesses/proofs.
+         
+      6) In the logic, we replace any 
+      
+               R v by [v] ∈ r
+
+         encoded according to the above description.
+
+      *)
+
+  (** We have computed the transitive closure, spec'ed and proved finite *)  
+
+  Variable (X : Type) (Xfin : finite_t X) (Xdiscr : discrete X) (x0 : X) (nt : nat).
+
+  Infix "∈" := hfs_mem.
+  Notation "x ⊆ y" := (forall u, u ∈ x -> u ∈ y).
+  Notation "⟬ x , y ⟭" := (hfs_opair x y).
+
+  Let X_surj_hfs : { l : hfs & { f : hfs -> X & 
+                    { g : X -> hfs |
+                      hfs_transitive l
+                   /\ (forall p, g p ∈ l)
+                   /\ (forall x, x ∈ l -> exists p, x = g p)
+                   /\ (forall p, f (g p) = p) } } }.
+  Proof.
+    destruct (finite_t_discrete_bij_t_pos Xfin)
+      as ([ | n ] & Hn); auto.
+    1: { exfalso; destruct Hn as (f & g & H1 & H2).
+         generalize (f x0); intro p; invert pos p. }
+    destruct Hn as (f & g & H1 & H2).
+    destruct (hfs_pos_n_transitive n) 
+      as (l & g' & f' & G1 & G2 & G3 & G4).
+    exists l, (fun x => g (g' x)), (fun x => f' (f x)); msplit 3; auto.
+    + intros x Hx.
+      destruct (G3 x Hx) as (p & Hp).
+      exists (g p); rewrite H2; auto.
+    + intros p; rewrite G4; auto.
+  Qed.
+
+  (** First a surjective map from some transitive set l to X *)
+
+  Let l := projT1 X_surj_hfs.
+  Let s := projT1 (projT2 X_surj_hfs).
+  Let i := proj1_sig (projT2 (projT2 (X_surj_hfs))).
+
+  Let Hl : hfs_transitive l.
+  Proof. apply (proj2_sig (projT2 (projT2 (X_surj_hfs)))). Qed.
+  Let Hs : forall x, s (i x) = x. 
+  Proof. apply (proj2_sig (projT2 (projT2 (X_surj_hfs)))). Qed.
+  Let Hi : forall x, i x ∈ l. 
+  Proof. apply (proj2_sig (projT2 (projT2 (X_surj_hfs)))). Qed.
+  Let Hi' : forall s, s ∈ l -> exists x, s = i x.
+  Proof. apply (proj2_sig (projT2 (projT2 (X_surj_hfs)))). Qed.
+
+  (** Now we build P^5 l that contains all the set of triples of l *)
+
+  Let p := iter hfs_pow l (2+(2*nt)).
+
+  Let Hp1 : hfs_transitive p.
+  Proof. apply hfs_iter_pow_trans; auto. Qed.
+
+  Let Hp2 : l ∈ p.
+  Proof.
+    apply hfs_iter_pow_le with (n := 1); simpl; auto; try lia.
+    apply hfs_pow_spec; auto.
+  Qed.
+
+  Let Hp3 x y : x ∈ l -> y ∈ l -> ⟬x,y⟭  ∈ iter hfs_pow l 2.
+  Proof.
+    intros Hx Hy.
+    do 2 apply hfs_pair_pow; auto.
+  Qed.
+
+  Let Hp4 x y : x ∈ l -> y ∈ l -> ⟬x,y⟭  ∈ p.
+  Proof.
+    intros Hx Hy.
+    generalize (Hp3 Hx Hy).
+    apply hfs_iter_pow_le; auto; lia.
+  Qed.
+
+  Let Hp5 n v : (forall p, vec_pos v p ∈ l) -> @hfs_tuple n v ∈ iter hfs_pow l (1+2*n).
+  Proof.
+    rewrite iter_plus; intros H.
+    apply hfs_tuple_pow; auto.
+    + simpl; apply hfs_pow_spec; intro; rewrite hfs_empty_spec; tauto.
+    + apply hfs_iter_pow_trans; auto.
+    + intros q; simpl; apply hfs_pow_trans_incr; auto.
+  Qed.
+
+  Let Hp6 n v : n <= nt -> (forall p, vec_pos v p ∈ l) -> @hfs_tuple n v ∈ p.
+  Proof. 
+    intros L H; apply Hp5 in H.
+    revert H.
+    unfold p.
+    apply hfs_iter_pow_le; try lia; auto.
+  Qed.
+
+  Variable (R : vec X nt -> Prop).
+  Hypothesis HR : forall v, { R v } + { ~ R v }.
+
+  Hint Resolve finite_t_prod hfs_mem_fin_t.
+
+  (** We encode R as a subset of tuples of elements of l in p *)
+
+  Let encode_R : { r | r ∈ p 
+                      /\ (forall v, @hfs_tuple nt v ∈ r -> forall q, vec_pos v q ∈ l)
+                      /\ forall v, R v <-> hfs_tuple (vec_map i v) ∈ r }.
+  Proof.
+    set (P v := R (vec_map s v) /\ forall q, vec_pos v q ∈ l).
+    set (f := @hfs_tuple nt). 
+    destruct hfs_comprehension with (P := P) (f := f) as (r & Hr).
+    + apply fin_t_dec.
+      * intros; apply HR.
+      * apply fin_t_vec with (P := fun t => t ∈ l).
+        apply hfs_mem_fin_t.
+    + exists r; msplit 2.
+      * unfold p. 
+        replace (2+2*nt) with ((1+2*nt)+1) by lia.
+        rewrite iter_plus with (b := 1).
+        apply hfs_pow_spec; intros x; rewrite Hr.
+        intros (v & H1 & <-).
+        apply Hp5, H1.
+      * unfold f; intros v.
+        rewrite Hr.
+        intros (w & H1 & H2).
+        apply hfs_tuple_spec in H2; subst w.
+        apply H1.
+      * intros v.
+        rewrite Hr.
+        split.
+        - exists (vec_map i v); split; auto.
+          split; auto.
+          ++ rewrite vec_map_map.
+             revert H; apply fol_equiv_ext.
+             f_equal; apply vec_pos_ext; intro; rew vec.
+          ++ intro; rew vec.
+        - intros (w & (H1 & _) & H2).
+          apply hfs_tuple_spec in H2.
+          revert H1; subst w; apply fol_equiv_ext.
+          f_equal; apply vec_pos_ext; intro; rew vec.
+  Qed.
+
+  Let r := proj1_sig encode_R.
+  
+  Let Hr1 : r ∈ p.
+  Proof. apply (proj2_sig encode_R). Qed.
+
+  Let Hr2 v : @hfs_tuple nt v ∈ r -> forall q, vec_pos v q ∈ l.
+  Proof. apply (proj2_sig encode_R). Qed.
+
+  Let Hr3 v : R v <-> hfs_tuple (vec_map i v) ∈ r.
+  Proof. apply (proj2_sig encode_R). Qed.
+
+  (** The Boolean encoding of x ∈ p *)
+
+  Let p_bool x := if hfs_mem_dec x p then true else false.
+
+  Let p_bool_spec x : x ∈ p <-> p_bool x = true.
+  Proof.   
+    unfold p_bool.
+    destruct (hfs_mem_dec x p); split; try tauto; discriminate.
+  Qed.
+
+  Let Y := sig (fun x => p_bool x = true).
+
+  Let eqY : forall x y : Y, proj1_sig x = proj1_sig y -> x = y.
+  Proof. 
+    intros (x & Hx) (y & Hy); simpl.
+    intros; subst; f_equal; apply UIP_dec, bool_dec.
+  Qed.
+
+  Let HY : finite_t Y.
+  Proof. 
+    apply fin_t_finite_t.
+    + intros; apply UIP_dec, bool_dec.
+    + generalize (hfs_mem_fin_t p); apply fin_t_equiv.
+      intros x; auto.
+  Qed.
+
+  Let discrY : discrete Y.
+  Proof.
+    intros (x & Hx) (y & Hy).
+    destruct (hfs_eq_dec x y) as [ -> | D ].
+    + left; f_equal; apply UIP_dec, bool_dec.
+    + right; contradict D; inversion D; auto.
+  Qed.
+
+  Let mem (x y : Y) := proj1_sig x ∈ proj1_sig y.
+
+  Let mem_dec : forall x y, { mem x y } + { ~ mem x y }.
+  Proof.
+    intros (a & ?) (b & ?); unfold mem; simpl; apply hfs_mem_dec.
+  Qed.
+
+  Let yl : Y.    Proof. exists l; apply p_bool_spec, Hp2. Defined.
+  Let yr : Y.    Proof. exists r; apply p_bool_spec, Hr1. Defined.
+
+  (** Membership equivalence is identity in the model *)
+
+  Let is_equiv : forall x y, mb_equiv mem x y <-> proj1_sig x = proj1_sig y.
+  Proof.
+    intros (x & Hx) (y & Hy); simpl.
+    unfold mb_equiv, mem; simpl; split.
+    2: intros []; tauto.
+    intros H.
+    apply hfs_mem_ext.
+    intros z; split; intros Hz.
+    * apply p_bool_spec in Hx.
+      generalize (Hp1 Hz Hx).
+      rewrite p_bool_spec; intros H'.
+      apply (H (exist _ z H')); auto.
+    * apply p_bool_spec in Hy.
+      generalize (Hp1 Hz Hy).
+      rewrite p_bool_spec; intros H'.
+      apply (H (exist _ z H')); auto.
+  Qed.
+
+  Let is_pair : forall x y k, mb_is_pair mem k x y 
+                          <-> proj1_sig k = hfs_pair (proj1_sig x) (proj1_sig y).
+  Proof.
+    intros (x & Hx) (y & Hy) (k & Hk); simpl.
+    unfold mb_is_pair; simpl; rewrite hfs_mem_ext.
+    generalize Hx Hy Hk; revert Hx Hy Hk.
+    do 3 rewrite <- p_bool_spec at 1.
+    intros Hx' Hy' Hk' Hx Hy Hk.
+    split.
+    + intros H a; split; rewrite hfs_pair_spec; [ intros Ha | intros [ Ha | Ha ] ].
+      * generalize (Hp1 Ha Hk'); rewrite p_bool_spec; intros Ha'.
+        specialize (H (exist _ a Ha')); simpl in H.
+        repeat rewrite is_equiv in H; apply H; auto.
+      * subst; apply (H (exist _ x Hx)); repeat rewrite is_equiv; simpl; auto.
+      * subst; apply (H (exist _ y Hy)); repeat rewrite is_equiv; simpl; auto.
+    + intros H (a & Ha); repeat rewrite is_equiv; simpl; rewrite <- hfs_pair_spec.
+      apply H.
+  Qed.
+ 
+  Let is_opair : forall x y k, mb_is_opair mem k x y 
+                           <-> proj1_sig k = ⟬proj1_sig x,proj1_sig y⟭.
+  Proof.
+    intros (x & Hx) (y & Hy) (k & Hk); simpl.
+    unfold mb_is_opair; split.
+    + intros ((a & Ha) & (b & Hb) & H); revert H.
+      repeat rewrite is_pair; simpl.
+      intros (-> & -> & ->); auto.
+    + intros ->.
+      generalize Hx Hy Hk; revert Hx Hy Hk.
+      do 3 rewrite <- p_bool_spec at 1.
+      intros Hx' Hy' Hk' Hx Hy Hk.
+      apply hfs_trans_opair_inv in Hk'; auto.
+      do 2 rewrite p_bool_spec in Hk'.
+      destruct Hk' as (H1 & H2).
+      exists (exist _ (hfs_pair x x) H1).
+      exists (exist _ (hfs_pair x y) H2).
+      repeat rewrite is_pair; simpl; auto.
+  Qed.
+
+  Let is_tuple n : forall v t, @mb_is_tuple _ mem t n v 
+                           <-> proj1_sig t = hfs_tuple (vec_map (@proj1_sig _ _) v).
+  Proof.
+    induction n as [ | n IHn ]; intros v (t & Ht).
+    + vec nil v; clear v; simpl; split.
+      * intros H; apply hfs_mem_ext.
+        intros z; split.
+        - intros Hz.
+          assert (Hz' : p_bool z = true).
+          { apply p_bool_spec.
+            apply Hp1 with (1 := Hz), p_bool_spec; auto. }
+          destruct (H (exist _ z Hz')); auto.
+        - rewrite hfs_empty_spec; tauto. 
+      * intros -> (z & ?); unfold mem; simpl.
+        rewrite hfs_empty_spec; tauto.
+    + vec split v with x; simpl; split.
+      * intros (t' & H1 & H2).
+        rewrite IHn in H2; try lia.
+        rewrite <- H2.
+        apply is_opair with (k := exist _ t Ht); auto.
+      * intros ->.
+        assert (H1 : p_bool (hfs_tuple (vec_map (@proj1_sig _ _) v)) = true).
+        { apply p_bool_spec.
+          apply p_bool_spec in Ht.
+          apply hfs_trans_opair_inv, proj2, hfs_trans_pair_inv in Ht; tauto. }
+        exists (exist _ (hfs_tuple (vec_map (@proj1_sig _ _) v)) H1); split.
+        - rewrite is_opair; simpl; auto.
+        - rewrite IHn; simpl; auto.
+  Qed.
+
+  Let has_tuples : mb_has_tuples mem yl nt.
+  Proof.
+    intros v Hv.
+    set (t := hfs_tuple (vec_map (proj1_sig (P:=fun x : hfs => p_bool x = true)) v)).
+    assert (H1 : p_bool t = true).
+    { apply p_bool_spec, Hp6; auto; intro; rew vec; apply Hv. }
+    exists (exist _ t H1).
+    apply is_tuple; simpl; reflexivity.
+  Qed.
+
+  Let i' : X -> Y.
+  Proof.
+    intros x.
+    exists (i x).
+    apply p_bool_spec.
+    generalize (Hi x) Hp2; apply Hp1.
+  Defined.
+
+  Let Hi'' x : mem (i' x) yl.
+  Proof. unfold i', yl, mem; simpl; auto. Qed.
+
+  Let s' (y : Y) : X := s (proj1_sig y).
+
+  (**
+    For finite and discrete type X, non empty (as witnessed by a given element)
+    equipped with a Boolean ternary relation R, one can compute a type Y, finite
+    and discrete, equipped with a Boolean binary membership predicate ∈ which is 
+    extensional. Y is a finite (set like) model which contains two sets yl and 
+    yr and there is a bijection between X and (the elements of) yl. All ordered 
+    triples build from elements of yl exist in Y, and yr encodes R in the set 
+    of (ordered) triples it contains. 
+    Finally, membership equivalence (≈) is the same as identity (=) in Y.
+
+    Membership equivalence : x ≈ y := ∀z, z∈x <-> z∈y
+    Membership extensional : x ≈ y -> ∀z, x∈z -> y∈z
+
+    Triples are build the usual way (in set theory)
+      - z ∈ {x,y} := z ≈ x \/ z ≈ y
+      - ordered pairs: (x,y) is {{x},{x,y}}
+      - ordered triples: (x,y,z) is ((x,y),z)
+
+    Non-emptyness is not really necessary but then bijection between X=ø and yl
+    has to be implemented with dependent functions, more cumbersome to work
+    with. And first order models can never be empty because one has to be able
+    to interpret variables. Maybe a discussion on the case of empty models
+    could be necessary, the logic been reduced to True/False in that case.
+    Any ∀ formula is True, any ∃ is False and no atomic formula can ever
+    be evaluated (because it contains terms that cannot be interpreted). 
+    Only closed formula have a meaning in the empty model 
+  *)
+  
+  Theorem reln_hfs : { Y : Type &
+                     { _ : finite_t Y & 
+                     { _ : discrete Y &
+                     { mem : Y -> Y -> Prop &
+                     { _ : forall u v, { mem u v } + { ~ mem u v } & 
+                     { yl : Y &
+                     { yr : Y & 
+                     { i : X -> Y & 
+                     { s : Y -> X &
+                             mb_member_ext mem
+                          /\ mb_has_tuples mem yl nt
+                          /\ (forall x, mem (i x) yl)
+                          /\ (forall y, mem y yl -> exists x, y = i x)
+                          /\ (forall x, s (i x) = x)
+                          /\ (forall v, R v <-> mb_is_tuple_in mem yr (vec_map i v))
+                          /\ (forall x y, mb_equiv mem x y <-> x = y)
+                      }}}}}}}}}.
+  Proof.
+    exists Y, HY, discrY, mem, mem_dec, yl, yr, i', s'.
+    msplit 6; auto.
+    + intros (u & Hu) (v & Hv) (w & Hw); unfold mem; simpl.
+      unfold mb_equiv; simpl; intros H.
+      cut (u = v); [ intros []; auto | ].
+      apply hfs_mem_ext.
+      apply p_bool_spec in Hu.
+      apply p_bool_spec in Hv.
+      clear w Hw.
+      intros x; split; intros Hx.
+      * generalize (Hp1 Hx Hu); rewrite p_bool_spec; intros H'.
+        apply (H (exist _ x H')); auto.
+      * generalize (Hp1 Hx Hv); rewrite p_bool_spec; intros H'.
+        apply (H (exist _ x H')); auto.
+    + intros y Hy; unfold i'.
+      destruct (Hi' Hy) as (x & Hx).
+      exists x; apply eqY; simpl; auto.
+    + intros v; rewrite Hr3; split.
+      * intros Hv.
+        red.
+        assert (H1 : p_bool (hfs_tuple (vec_map i v)) = true).
+        { apply p_bool_spec, Hp1 with (1 := Hv); auto. }
+        exists (exist _ (hfs_tuple (vec_map i v)) H1); split.
+        - apply is_tuple; simpl; rewrite vec_map_map; auto.
+        - unfold yr; red; simpl; auto.
+      * intros ((t & Ht) & H1 & H2).
+        rewrite is_tuple in H1.
+        simpl in H1, H2.
+        rewrite vec_map_map in H1; subst t.
+        apply H2. 
+    + intros x y; rewrite is_equiv; split; auto.
+      intros; subst; auto.
+  Qed.
+
+End bt_model_n.
+
